Play with preliminary setup for big-step interpreter

vyperInterpreterScript.sml
@@ -1,7 +1,7 @@
-open HolKernel boolLib bossLib Parse wordsLib dep_rewrite
-     finite_mapTheory
+open HolKernel boolLib bossLib Parse wordsLib blastLib dep_rewrite
+     byteTheory finite_mapTheory
      cv_typeTheory cv_stdTheory cv_transLib
-open vfmTypesTheory vyperAstTheory
+open vfmTypesTheory vfmStateTheory vyperAstTheory
 
 val () = new_theory "vyperInterpreter";
 
@@ -65,6 +65,57 @@ Proof
   \\ gvs[Q.SPEC`Pair x y`cv_size'_def]
 QED
 
+Theorem set_byte_160:
+  set_byte a b (w: 160 word) be =
+  let i = byte_index a be in
+       if i =   0 then w2w b        || w && 0xFFFFFFFFFFFFFFFFFFFFFFFFFFFFFFFFFFFFFF00w
+  else if i =   8 then w2w b <<   8 || w && 0xFFFFFFFFFFFFFFFFFFFFFFFFFFFFFFFFFFFF00FFw
+  else if i =  16 then w2w b <<  16 || w && 0xFFFFFFFFFFFFFFFFFFFFFFFFFFFFFFFFFF00FFFFw
+  else if i =  24 then w2w b <<  24 || w && 0xFFFFFFFFFFFFFFFFFFFFFFFFFFFFFFFF00FFFFFFw
+  else if i =  32 then w2w b <<  32 || w && 0xFFFFFFFFFFFFFFFFFFFFFFFFFFFFFF00FFFFFFFFw
+  else if i =  40 then w2w b <<  40 || w && 0xFFFFFFFFFFFFFFFFFFFFFFFFFFFF00FFFFFFFFFFw
+  else if i =  48 then w2w b <<  48 || w && 0xFFFFFFFFFFFFFFFFFFFFFFFFFF00FFFFFFFFFFFFw
+  else if i =  56 then w2w b <<  56 || w && 0xFFFFFFFFFFFFFFFFFFFFFFFF00FFFFFFFFFFFFFFw
+  else if i =  64 then w2w b <<  64 || w && 0xFFFFFFFFFFFFFFFFFFFFFF00FFFFFFFFFFFFFFFFw
+  else if i =  72 then w2w b <<  72 || w && 0xFFFFFFFFFFFFFFFFFFFF00FFFFFFFFFFFFFFFFFFw
+  else if i =  80 then w2w b <<  80 || w && 0xFFFFFFFFFFFFFFFFFF00FFFFFFFFFFFFFFFFFFFFw
+  else if i =  88 then w2w b <<  88 || w && 0xFFFFFFFFFFFFFFFF00FFFFFFFFFFFFFFFFFFFFFFw
+  else if i =  96 then w2w b <<  96 || w && 0xFFFFFFFFFFFFFF00FFFFFFFFFFFFFFFFFFFFFFFFw
+  else if i = 104 then w2w b << 104 || w && 0xFFFFFFFFFFFF00FFFFFFFFFFFFFFFFFFFFFFFFFFw
+  else if i = 112 then w2w b << 112 || w && 0xFFFFFFFFFF00FFFFFFFFFFFFFFFFFFFFFFFFFFFFw
+  else if i = 120 then w2w b << 120 || w && 0xFFFFFFFF00FFFFFFFFFFFFFFFFFFFFFFFFFFFFFFw
+  else if i = 128 then w2w b << 128 || w && 0xFFFFFF00FFFFFFFFFFFFFFFFFFFFFFFFFFFFFFFFw
+  else if i = 136 then w2w b << 136 || w && 0xFFFF00FFFFFFFFFFFFFFFFFFFFFFFFFFFFFFFFFFw
+  else if i = 144 then w2w b << 144 || w && 0xFF00FFFFFFFFFFFFFFFFFFFFFFFFFFFFFFFFFFFFw
+  else if i = 152 then w2w b << 152 || w && 0x00FFFFFFFFFFFFFFFFFFFFFFFFFFFFFFFFFFFFFFw
+  else                 w2w b << 160 || w && 0xFFFFFFFFFFFFFFFFFFFFFFFFFFFFFFFFFFFFFFFFw
+Proof
+  rw_tac std_ss [set_byte_def, word_slice_alt_def]
+  \\ reverse(rpt IF_CASES_TAC)
+  >- (
+    `i = 160`
+    by (
+      qunabbrev_tac`i`
+      \\ full_simp_tac (std_ss ++ boolSimps.LET_ss ++ ARITH_ss) [
+            byte_index_def, EVAL``dimindex(:160)``]
+      \\ `w2n a MOD 20 < 20` by rw[]
+      \\ pop_assum mp_tac
+      \\ qmatch_goalsub_abbrev_tac`z < 20 ⇒ f`
+      \\ simp_tac std_ss [wordsTheory.NUMERAL_LESS_THM]
+      \\ strip_tac \\ gs[Abbr`f`]
+      \\ rw[] \\ gs[] )
+    \\ asm_simp_tac std_ss []
+    \\ simp_tac (srw_ss()) []
+    \\ BBLAST_TAC)
+  \\ asm_simp_tac std_ss []
+  \\ simp_tac (srw_ss()) []
+  \\ BBLAST_TAC
+QED
+
+val () = cv_auto_trans set_byte_160;
+
+val () = cv_auto_trans (INST_TYPE [alpha |-> “:160”] word_of_bytes_def);
+
 (* -- *)
 
 Definition string_to_num_def:
@@ -86,7 +137,9 @@ End
 
 Overload AddressV = “λw: address. BytesV (Fixed 20) (word_to_bytes w T)”
 
-val from_to_value = cv_typeLib.from_to_thm_for “:value”;
+val from_to_value_thm = cv_typeLib.from_to_thm_for “:value”;
+val from_value = from_to_value_thm |> concl |> rator |> rand
+val to_value = from_to_value_thm |> concl |> rand
 
 Datatype:
   subscript
@@ -197,5 +250,217 @@ val () = cv_auto_trans_rec default_value_def (
   >- (IF_CASES_TAC \\ gs[cv_size'_cv_mk_BN])
   \\ IF_CASES_TAC \\ gs[]
 );
+
+(*
+We don't use this directly to support cv which prefers num keys
+Type scope = “:identifier |-> value”;
+*)
+Type scope = “:num |-> value”;
+
+Definition lookup_scopes_def:
+  lookup_scopes id [] = NONE ∧
+  lookup_scopes id ((env: scope)::rest) =
+  case FLOOKUP env id of NONE =>
+    lookup_scopes id rest
+  | SOME v => SOME v
+End
+
+Type containing_scope = “:scope list # scope # scope list”;
+
+Datatype:
+  location
+  = ScopedVar containing_scope identifier
+  | Global identifier
+End
+
+Datatype:
+  assignment_value
+  = BaseTargetV location (subscript list)
+  | TupleTargetV (assignment_value list)
+End
+
+Datatype:
+  exception
+  = RaiseException string
+  | AssertException string
+  | Error string
+  | BreakException
+  | ContinueException
+End
+
+Datatype:
+  result = Done α | Exc exception
+End
+
+Definition evaluate_literal_def:
+  evaluate_literal (BoolL b)   = BoolV b ∧
+  evaluate_literal (StringL n s) = StringV n s ∧
+  evaluate_literal (BytesL b bs) = BytesV b bs ∧
+  evaluate_literal (IntL i)    = IntV i
+End
+
+val () = cv_auto_trans evaluate_literal_def;
+
+Definition evaluate_binop_def:
+  evaluate_binop (Add:binop) (IntV i1) (IntV i2) = Done (IntV (i1 + i2)) ∧
+  evaluate_binop Sub (IntV i1) (IntV i2) = Done (IntV (i1 - i2)) ∧
+  evaluate_binop Mul (IntV i1) (IntV i2) = Done (IntV (i1 * i2)) ∧
+  evaluate_binop _ _ _ = Exc $ Error "binop"
+End
+
+val () = cv_auto_trans evaluate_binop_def;
+
+Definition evaluate_builtin_def:
+  evaluate_builtin _ Len [BytesV _ ls] = Done (IntV &(LENGTH ls)) ∧
+  evaluate_builtin _ Len [StringV _ ls] = Done (IntV &(LENGTH ls)) ∧
+  evaluate_builtin _ Len [ArrayV _ ls] = Done (IntV &(LENGTH ls)) ∧
+  evaluate_builtin _ Eq [StringV _ s1; StringV _ s2] = Done (BoolV (s1 = s2)) ∧
+  evaluate_builtin _ Eq [BytesV _ s1; BytesV _ s2] = Done (BoolV (s1 = s2)) ∧
+  evaluate_builtin _ Eq [BoolV b1; BoolV b2] = Done (BoolV (b1 = b2)) ∧
+  evaluate_builtin _ Eq  [IntV i1; IntV i2] = Done (BoolV (i1 = i2)) ∧
+  evaluate_builtin _ Lt  [IntV i1; IntV i2] = Done (BoolV (i1 < i2)) ∧
+  evaluate_builtin _ Not [BoolV b] = Done (BoolV (¬b)) ∧
+  evaluate_builtin _ (Bop bop) [v1; v2] = evaluate_binop bop v1 v2 ∧
+  evaluate_builtin bal (Acc Balance) [BytesV _ bs] =
+    (case ALOOKUP bal (word_of_bytes T (0w:address) bs) of
+          SOME n => Done (IntV &n)
+        | NONE => Exc $ Error "missing balance") ∧
+  evaluate_builtin _ _ _ = Exc $ Error "builtin"
+End
+
+val () = cv_auto_trans evaluate_builtin_def;
+
+Definition extract_elements_def:
+  extract_elements (ArrayV _ vs) = SOME vs ∧
+  extract_elements _ = NONE
+End
+
+val () = cv_auto_trans extract_elements_def;
+
+Definition replace_elements_def:
+  replace_elements (ArrayV b _) vs = SOME (ArrayV b vs) ∧
+  replace_elements _ _ = NONE
+End
+
+val () = cv_auto_trans replace_elements_def;
+
+Definition integer_index_def:
+  integer_index vs i =
+   if Num i < LENGTH vs then
+     SOME $ if 0 ≤ i then Num i else LENGTH vs - Num i
+   else NONE
+End
+
+val () = cv_auto_trans integer_index_def;
+
+Definition evaluate_subscript_def:
+  evaluate_subscript av (IntV i) =
+  (case extract_elements av of SOME vs =>
+    (case integer_index vs i of SOME j => Done (EL j vs)
+     | _ => Exc $ Error "integer_index")
+   | _ => Exc $ Error "extract_elements") ∧
+  evaluate_subscript _ _ = Exc $ Error "evaluate_subscript"
+End
+
+val evaluate_subscript_pre_def = cv_auto_trans_pre evaluate_subscript_def;
+
+Theorem evaluate_subscript_pre[cv_pre]:
+  evaluate_subscript_pre av v
+Proof
+  rw[evaluate_subscript_pre_def, integer_index_def]
+  \\ rw[]
+  \\ qmatch_asmsub_rename_tac`0i ≤ v0`
+  \\ Cases_on`v0` \\ gs[]
+QED
+
+Definition evaluate_attribute_def:
+  evaluate_attribute (StructV kvs) id =
+  (case ALOOKUP kvs id of SOME v => Done v
+   | _ => Exc $ Error "attribute") ∧
+  evaluate_attribute _ _ = Exc $ Error "evaluate_attribute"
+End
+
+val () = cv_auto_trans evaluate_attribute_def;
+
+Definition compatible_bound_def:
+  compatible_bound (Fixed n) m = (n = m) ∧
+  compatible_bound (Dynamic n) m = (m ≤ n)
+End
+
+val () = cv_auto_trans compatible_bound_def;
+
+Definition builtin_args_length_ok_def:
+  builtin_args_length_ok Len n = (n = 1n) ∧
+  builtin_args_length_ok Not n = (n = 1) ∧
+  builtin_args_length_ok Eq n = (n = 2) ∧
+  builtin_args_length_ok Lt n = (n = 2) ∧
+  builtin_args_length_ok (Bop _) n = (n = 2) ∧
+  builtin_args_length_ok (Msg _) n = (n = 0) ∧
+  builtin_args_length_ok (Acc _) n = (n = 1)
+End
+
+val () = cv_auto_trans builtin_args_length_ok_def;
+
+Datatype:
+  call_txn = <|
+    sender: address
+  ; target: address
+  ; function_name: identifier
+  ; args: value list
+  ; value: num
+  |>
+End
+
+Datatype:
+  evaluation_context = <|
+    env: scope list
+  ; stk: identifier list (* add loops *)
+  ; txn: call_txn
+  |>
+End
+
+Datatype:
+  contract = <|
+    src: toplevel list
+  ; globals: (* identifier *) num |-> toplevel_value
+  |>
+End
+
+Datatype:
+  evaluation_state = <|
+    contracts: (address, contract) alist
+  ; accounts: evm_accounts
+  |>
+End
+
+(*
+Definition evaluate_def:
+  eval_stmt cx st Pass = Done st ∧
+  eval_stmt cx st Continue
+*)
+
+Definition value_to_key_def:
+  value_to_key (IntV i) = SOME $ IntSubscript i ∧
+  value_to_key (StringV _ s) = SOME $ StrSubscript s ∧
+  value_to_key (BytesV _ bs) = SOME $ BytesSubscript bs ∧
+  value_to_key _ = NONE
+End
+
+val () = cv_auto_trans value_to_key_def;
+
+(* TODO: assumes unique identifiers, but should check? *)
+Definition initial_globals_def:
+  initial_globals env [] = FEMPTY ∧
+  initial_globals env (VariableDecl _ Storage id typ :: ts) =
+  initial_globals env ts |+ (string_to_num id, Value $ default_value env typ) ∧
+  initial_globals env (VariableDecl _ Transient id typ :: ts) =
+  initial_globals env ts |+ (string_to_num id, Value $ default_value env typ) ∧
+  (* TODO: handle Constants and  Immutables *)
+  initial_globals env (HashMapDecl _ id kt vt :: ts) =
+  initial_globals env ts |+ (string_to_num id, HashMap []) ∧
+  initial_globals env (t :: ts) = initial_globals env ts
+End
+
+val () = cv_auto_trans initial_globals_def;
 
 val () = export_theory();
